update FStar.Int64

src/Zulib/fstar/FStar.Int64.fst
@@ -1,58 +1,73 @@
 module FStar.Int64
 
-let n = 64
+unfold let n = 64
 
-open FStar.UInt
+open FStar.Int
 open Zen.Option
 
-private type t' = | Mk: v:uint_t n -> t'
-type t = t'
+abstract type t =
+    | Mk: v:int_t n -> t
 
-let v (x:t) : uint_t n = x.v
+abstract let v (x:t) : int_t n = x.v
 
-let v_inj (x1 x2: t): Lemma (requires (v x1 == v x2))
-                            (ensures (x1 == x2)) = ()
+abstract val int_to_t: x:int_t n -> Pure t
+  (requires True)
+  (ensures (fun y -> v y = x))
+abstract let int_to_t x = Mk x
 
-val add: a:t -> b:t -> Pure t
+let uv_inv (x : t) : Lemma
+  (ensures (int_to_t (v x) == x))
+  [SMTPat (v x)] = ()
+
+let vu_inv (x : int_t n) : Lemma
+  (ensures (v (int_to_t x) == x))
+  [SMTPat (int_to_t x)] = ()
+
+let v_inj (x1 x2: t): Lemma
+  (requires (v x1 == v x2))
+  (ensures (x1 == x2))
+  = ()
+
+abstract val add: a:t -> b:t -> Pure t
   (requires (size (v a + v b) n))
   (ensures (fun c -> v a + v b = v c))
-let add a b = Mk (add (v a) (v b))
+abstract let add a b = Mk (add (v a) (v b))
 
-val add_mod: a:t -> b:t -> Pure t
+abstract val add_mod: a:t -> b:t -> Pure t
   (requires True)
-  (ensures (fun c -> (v a + v b) % pow2 n = v c))
-let add_mod a b = Mk (add_mod (v a) (v b))
+  (ensures (fun c -> (v a + v b) @% pow2 n = v c))
+abstract let add_mod a b = Mk (add_mod (v a) (v b))
 
-val checked_add: a:t -> b:t -> option t
-let checked_add a b = map Mk (checked_add (v a) (v b))
+abstract val checked_add: a:t -> b:t -> option t
+abstract let checked_add a b = map Mk (checked_add (v a) (v b))
 
 (* Subtraction primitives *)
-val sub: a:t -> b:t -> Pure t
+abstract val sub: a:t -> b:t -> Pure t
   (requires (size (v a - v b) n))
   (ensures (fun c -> v a - v b = v c))
-let sub a b = Mk (sub (v a) (v b))
+abstract let sub a b = Mk (sub (v a) (v b))
 
-val sub_mod: a:t -> b:t -> Pure t
+abstract val sub_mod: a:t -> b:t -> Pure t
   (requires True)
-  (ensures (fun c -> (v a - v b) % pow2 n = v c))
-let sub_mod a b = Mk (sub_mod (v a) (v b))
+  (ensures (fun c -> (v a - v b) @% pow2 n = v c))
+abstract let sub_mod a b = Mk (sub_mod (v a) (v b))
 
-val checked_sub: a:t -> b:t -> option t
-let checked_sub a b = map Mk (checked_sub (v a) (v b))
+abstract val checked_sub: a:t -> b:t -> option t
+abstract let checked_sub a b = map Mk (checked_sub (v a) (v b))
 
 (* Multiplication primitives *)
-val mul: a:t -> b:t -> Pure t
+abstract val mul: a:t -> b:t -> Pure t
   (requires (size (v a * v b) n))
   (ensures (fun c -> v a * v b = v c))
-let mul a b = Mk (mul (v a) (v b))
+abstract let mul a b = Mk (mul (v a) (v b))
 
-val mul_mod: a:t -> b:t -> Pure t
+abstract val mul_mod: a:t -> b:t -> Pure t
   (requires True)
-  (ensures (fun c -> (v a * v b) % pow2 n = v c))
-let mul_mod a b = Mk (mul_mod (v a) (v b))
+  (ensures (fun c -> (v a * v b) @% pow2 n = v c))
+abstract let mul_mod a b = Mk (mul_mod (v a) (v b))
 
-val checked_mul: a:t -> b:t -> option t
-let checked_mul a b = map Mk (checked_mul (v a) (v b))
+abstract val checked_mul: a:t -> b:t -> option t
+abstract let checked_mul a b = map Mk (checked_mul (v a) (v b))
 
 (*
 val mul_div: a:t -> b:t -> Pure t
@@ -62,20 +77,20 @@ let mul_div a b = Mk (mul_div (v a) (v b))
 *)
 
 (* Division primitives *)
-val div: a:t -> b:t{v b <> 0} -> Pure t
-  (requires (True))
-  (ensures (fun c -> v b <> 0 ==> v a / v b = v c))
-let div a b = Mk (div (v a) (v b))
+abstract val div: a:t -> b:t{v b <> 0} -> Pure t
+  (requires (size (v a / v b) n))
+  (ensures (fun c -> v a / v b = v c))
+abstract let div a b = Mk (div (v a) (v b))
 
-val checked_div: a:t -> b:t -> option t
-let checked_div a b = map Mk (checked_div (v a) (v b))
+abstract val checked_div: a:t -> b:t -> option t
+abstract let checked_div a b = map Mk (checked_div (v a) (v b))
 
 (* Modulo primitives *)
-val rem: a:t -> b:t{v b <> 0} -> Pure t
+abstract val rem: a:t -> b:t{v b <> 0} -> Pure t
   (requires True)
   (ensures (fun c ->
     v a - ((v a / v b) * v b) = v c))
-let rem a b = Mk (mod (v a) (v b))
+abstract let rem a b = Mk (mod (v a) (v b))
 
 (*
 (* Bitwise operators *)
@@ -87,37 +102,6 @@ val logor: t -> t -> Tot t
 let logor a b = Mk (logor (v a) (v b))
 val lognot: t -> Tot t
 let lognot a = Mk (lognot (v a))
-*)
-val uint_to_t: x:uint_t n -> Pure t
-  (requires True)
-  (ensures (fun y -> v y = x))
-let uint_to_t x = Mk x
-
-#set-options "--lax"
-//This private primitive is used internally by the
-//compiler to translate bounded integer constants
-//with a desugaring-time check of the size of the number,
-//rather than an expensive verifiation check.
-//Since it is marked private, client programs cannot call it directly
-//Since it is marked unfold, it eagerly reduces,
-//eliminating the verification overhead of the wrapper
-private
-unfold
-let __uint_to_t (x:int) : t
-    = uint_to_t x
-#reset-options
-
-(*
-(* Shift operators *)
-val shift_right: a:t -> s:UInt32.t -> Pure t
-  (requires True)
-  (ensures (fun c -> UInt32.v s < n ==> v c = (v a / (pow2 (UInt32.v s)))))
-let shift_right a s = Mk (shift_right (v a) (UInt32.v s))
-
-val shift_left: a:t -> s:UInt32.t -> Pure t
-  (requires True)
-  (ensures (fun c -> UInt32.v s < n ==> v c = ((v a * pow2 (UInt32.v s)) % pow2 n)))
-let shift_left a s = Mk (shift_left (v a) (UInt32.v s))
 *)
 
 (* Comparison operators *)
